#+TITLE: Methods of Inference
#+AUTHOR: Nathan Moos
#+DATE: 2015-09-17
#+LATEX_HEADER: \newcommand*\myline{\rule{0.5cm}{0.4pt}}

* Definitions

- Argument :: is a sequence of statements ending in a conclusion
- Premises :: Statements assumed to be true at the beginning.
- Valid argument :: Does the conclusion follow from the premises?
- True argument :: If the premises are true, the conclusion must also be true.
                  
A common notation is
\begin{align*}
&p_1 \\
&p_2 \\
&p_3 \\
&\myline \\
\therefore &q
\end{align*}

If the argument is valid, $(p_1 \land p_2 \land p_3) \implies q$ is a tautology.

* Rules of Inference

** /Modus ponens/

\begin{align*}
&p \implies q \\
&p \\
&\rule{0.5cm}{0.4pt} \\
\therefore &q
\end{align*}

** /Modus tollens/

\begin{align*}
&p \implies q \\
&\lnot q \\
&\myline \\
\therefore &\lnot p
\end{align*}

** Resolution
   
\begin{align*}
&p \lor q \\
&\lnot p \lor r \\
&\myline \\
\therefore &q \lor r
\end{align*}

** Hypothetical syollogism
   
\begin{align*}
&p \implies q \\
&q \implies r \\
&\myline \\
\therefore &p \implies r
\end{align*}

** Addition
   
\begin{align*}
&p \\
&\myline \\
\therefore &p \lor q
\end{align*}

** Disjunctive syllogism
   
\begin{align*}
&p \lor q \\
&\lnot p \\
&\myline \\
\therefore &q
\end{align*}

** Simplification

\begin{align*}
&p \land q \\
&\myline \\
\therefore &p
\end{align*}

** Conjunction

\begin{align*}
&p \\
&q \\
&\myline \\
\therefore &p \land q
\end{align*}

* Fallacies

** Affirming the conclusion
   
\begin{align*}
&p \implies q \\
&q \\
&\myline \\
\therefore &p
\end{align*}

** Denying the hypothesis

\begin{align*}
&p \implies q \\
&\lnot p \\
&\myline \\
\therefore &q
\end{align*}

* Inference with quantifiers
  
** Universal instantiation

\begin{align*}
&\forall x P(x) \\
&\myline \\
\therefore &P(C) \text{ for any arbitrary $C$.}
\end{align*}

** Universal generalization

The converse of universal instantiation.

** Existential instantiation

\begin{align*}
&\exists x P(x) \\
&\myline \\
\therefore &P(C) \text{ for some $C$.}
\end{align*}

** Existential generalization

The converse of existential instantiation.

* Building a valid argument 
  
** Without quantifiers
  
Say we have the following:
\begin{align}
&B \implies A \\
&S \iff (A \land \lnot y) \\
&B \\
&\lnot y \\
\nonumber &\myline \\
\nonumber \therefore &S
\end{align}

The following steps let us prove it:

1. $A$ is true by /modus ponens/ of (1), (3).
2. $A \land \lnot y$ is true by conjunction of (1), (4).
4. $(A \land \lnot y) \implies S$ is true by definition of $\iff$ 
   and simplification of (2).
5. Therefore, $S$ by /modus ponens/ applied to $2$ and $4$.

** With quantifiers

Say we have:
\begin{align}
&\forall x (B(x) \implies A(x)) \\
&\exists x B(x) \\
\nonumber &\myline \\
\nonumber \therefore &\exists x A(x)
\end{align}

1. $B(C)$ by existential instantiation of (2)
2. $B(C) \implies A(C)$ by universal instantiation of (1)
3. $A(C)$ by /modus ponens/ of steps 1 and 2.
4. $\exists x A(x)$ by existential generalization of step 3.
* Methods of proof

** Direct proof

Show that $p \implies q$.

** Proof  by contraposition

Instead of trying to prove $p \implies q$, prove that $\lnot q \implies \lnot
p$. Those two are logical equivalences.

This is very helpful for a large number of premises.

$$ p_1 \iff p_2 \iff p_3 \iff ... \iff p_n \equiv (p_1 \implies p_2) \land
   (p_2 \implies p_3) \land ... \land (p_n \implies p_1) $$
   
A proof by contraposition can simplify the sub-proofs.
