#+TITLE: Mathematical Induction
#+AUTHOR: Nathan Moos
#+DATE: 2015-10-06
#+LATEX_HEADER: \newcommand*\Z{\mathbb{Z}}
#+LATEX_HEADER: \newcommand*\R{\mathbb{R}}
#+LATEX_HEADER: \newcommand*\ret{\rightarrow}

* Definition

Let $P(n)$ be a predicate defined $\forall n \in \Z^+$. The principle of
mathematical induction is that if $P(1)$ and $P(k) \implies P(k + 1)$
$\forall k \in \Z^+$, then $P(n)$ is true $\forall n \in \Z^+$.

$$ P(1) \land \forall k \in \Z^+ (P(k) \implies P(k + 1)) \implies \forall n \in \Z^+ P(n)$$

Induction can also be used to prove /inequalities/.

* Proof Form

- Base step :: $P(1)$
- Inductive step :: $\forall k \in \Z^+ (P(k) \implies P(k+1))$
- Conclusion :: $\forall n \in \Z^+ P(n)$

** Inductive step

Assume $P(k)$ is true, then show that $P(k+1)$ is true. This seems backwards --
circular reasoning much? Not really, all we want to show is that *if* $P(k)$,
*then* $P(k+1)$.

* Example

Find the formula for $a_n = \frac{1}{1 \cdot 4} + \frac{1}{4 \cdot 7} + ... + \frac{1}{(3n - 2)(3n + 1)}$
and prove it $\forall n \in \Z^+$.

*Step 1:* Write it out:
\begin{align*}
a_1 &= \frac{1}{4} \\
a_2 &= \frac{2}{7} \\
a_3 &= \frac{3}{10} \\
a_4 &= \frac{4}{13} \\
\implies a_n &= \frac{n}{3n + 1}
\end{align*}

** Proof by induction

*Step 2:* Base case:
\begin{align*}
a_1 &= \frac{1}{3(1) + 1} \\
&= \frac{1}{3 + 1} \\
&= \frac{1}{4} \\
&= a_1
\end{align*}

*Step 3:* Inductive step:
\begin{align*}
a_k &= \frac{k}{3k + 1} \\
a_{k+1} &= \frac{k + 1}{3(k + 1) + 1} \\
&= \frac{k + 1}{3k + 4} \\
a_{k+1} &= a_k + \frac{1}{(3(k + 1) - 2)(3(k + 1) + 1)} \\
&= \frac{k}{3k + 1} + \frac{1}{(3k + 1)(3k + 4)} \\
&= \frac{k(3k + 4) + 1}{(3k + 1)(3k + 4)} \\
&= \frac{k + 1}{3k + 4} \\
&= a_{k+1}
\end{align*}
